revert changes to ValList

src/InterParse.v
@@ -966,9 +966,27 @@ Module InterParse.
       | Some f, Some v => Some v (* Include everything else, type checking later in the serializer process *)
       end.
 
-    Definition ValList (d : Desc) (v : Value) : list (Z * Val) :=
+    Definition ValList' (d : Desc) (v : Value) : list (Z * Val) :=
       map_to_list (merge Filter (Fields d) (Vals v)).
-      
+    
+    Definition ValList_filter_p (d : Desc) (kv : Z * Val) : Prop :=
+      match (Fields d) !! (fst kv), (snd kv) with
+      | Some _, V_MISSING => False
+      | None, _ => False
+      | _, _ => True
+      end.
+
+    Global Instance ValList_filter_Decision (d : Desc) : forall kv : Z * Val, Decision (ValList_filter_p d kv).
+    Proof.
+      intros [k v].
+      unfold ValList_filter_p, fst, snd.
+      destruct (Fields d !! k); last apply False_dec.
+      destruct v; (apply True_dec || apply False_dec).
+    Defined.
+
+    Definition ValList (d : Desc) (v : Value) : list (Z * Val) :=
+      filter (ValList_filter_p d) (map_to_list (Vals v)).
+  
     Definition field_val_match (f : Field) (v : Val) : Prop :=
       match v, f with
       | V_BOOL _, F_BOOL
@@ -1241,11 +1259,11 @@ Module InterParse.
     Qed.
 
     Lemma kv_in_Filter : forall vs d key val,
-      (key, val) ∈ ValList d (VALUE vs) -> 
+      (key, val) ∈ ValList' d (VALUE vs) -> 
       (key, val) ∈ map_to_list vs.
     Proof.
       intros vs d key val.
-      unfold ValList, Vals.
+      unfold ValList', Vals.
       intros Hfilter.
       rewrite elem_of_map_to_list. 
       rewrite elem_of_map_to_list in Hfilter.
@@ -1287,7 +1305,9 @@ Module InterParse.
       unfold S.Bind', S.Concat, S.Len'.
       (* Show that both decide expressions evaluate to true *)
       unfold ValList, Vals in Hin.
-      apply kv_in_Filter in Hin.
+      rewrite list_elem_of_filter in Hin.
+      destruct Hin as [Hfilter Hin].
+      (* apply kv_in_Filter in Hin. *)
       rewrite elem_of_map_to_list in Hin.
       pose proof (ValueDepthDropFirst k v m Hnone Hfst) as Hdepth. 
       destruct (decide (ValueDepth val < ValueDepth (VALUE m))%nat) eqn:Hm.
@@ -1299,24 +1319,6 @@ Module InterParse.
           destruct (ValueDepth val == ValueDepth (VALUE m)),
                      (ValueDepth val == ValueDepth (VALUE (<[k := v]> m))); done.
     Qed.
-
-    Lemma insert_merge_r_conditional : 
-      ∀ {K : Type} {M : Type → Type} {H : FMap M} {H0 : ∀ A : Type, Lookup K A (M A)}
-        {H1 : ∀ A : Type, Empty (M A)} {H2 : ∀ A : Type, PartialAlter K A (M A)} {H3 : OMap M}
-        {H4 : base.Merge M} {H5 : ∀ A : Type, MapFold K A (M A)} {EqDecision0 : EqDecision K},
-      FinMap K M
-      → ∀ {A B C : Type} (f : option A → option B → option C) (m1 : M A) (m2 : M B) (i : K) (x : C) (z : B),
-      merge f m1 (<[i:=z]> m2) = match (f (m1 !! i) (Some z)) with
-                                 | Some x => <[i:=x]> (merge f m1 m2)
-                                 | None => merge f (delete i m1) m2
-                                 end.
-    Proof.
-      intros.
-      destruct (f (m1 !! i) (Some z)) eqn:Hfeq.
-      - symmetry. apply partial_alter_merge_r. unfold diag_None.
-        destruct (m1 !! i); by rewrite Hfeq.
-      - symmetry.
-    Admitted.
 
     Lemma SerialValueInversion (d : Desc) :
       forall k v (m : gmap Z Val) enc,
@@ -1331,8 +1333,6 @@ Module InterParse.
       - unfold SerialValue at 1, S.RecursiveState.
         rewrite ser_recur_st_unfold.
         unfold SerialValue', S.Map, ValList, Vals.
-      Admitted.
-    (*
         rewrite map_to_list_insert_first_key by assumption.
         rewrite filter_cons.
         destruct (decide (ValList_filter_p d (k, v))) as [Hfilter_in | Hfilter_out].
@@ -1483,7 +1483,6 @@ Module InterParse.
             rewrite SerialRepSubst; first reflexivity.
             apply SerialValWeakenDepth; assumption.
     Qed.
-     *)
 
     Definition ValueEncLength_P (v : Value) :=
       forall d enc,
@@ -1505,9 +1504,8 @@ Module InterParse.
       - (* Prove the main statement about Values, using nested induction. *)
         revert IHv. induction vs as [| k v m Hno Hfst ] using map_first_key_ind.
         + intros _ d enc Hvalid Hser.
-          (* vm_compute in Hser. *)
-          (* inversion Hser. destruct d; reflexivity. *)
-          admit.
+          vm_compute in Hser.
+          inversion Hser. destruct d; reflexivity.
         + intros IHv d enc Hvalid Hser; unfold S.Output in *. 
           apply SerialValueInversion in Hser; try assumption.
           destruct Hser as (enc__v & enc__rest & Hrest_ok & Hv_ok & Henc).
@@ -1575,7 +1573,7 @@ Module InterParse.
         destruct (fs !! k).
         + destruct f; try discriminate; (intros Hv_ok; invc Hv_ok; apply Length_default).
         + intros Hv_ok; invc Hv_ok; apply Length_default.
-    Admitted.
+    Qed.
 
     Lemma WillEncode_NonEmpty :
       forall d k v enc,
@@ -2162,8 +2160,6 @@ Module InterParse.
     Proof.
       intros f Hnone.
       unfold ValList, Vals.
-    Admitted.
-    (*
       apply list_filter_iff_local.
       intros [k' v'] Hin.
       split.
@@ -2178,7 +2174,6 @@ Module InterParse.
         + subst k. rewrite Hin in Hnone. discriminate.
         + rewrite lookup_insert_ne by done. done.
     Qed.
-     *)
 
     Lemma SC_filter : forall v d, ⟨ v ∷ d ⟩ -> ValList d v = map_to_list (Vals v).
     Proof.
@@ -2186,7 +2181,7 @@ Module InterParse.
       unfold ValList, Vals.
       intros d Hsc. apply SC_SCO in Hsc.
       dependent induction Hsc.
-      - simpl. by rewrite merge_empty, map_to_list_empty.
+      - by rewrite map_to_list_empty, filter_nil.
       - rename H into Hty,
                  H0 into Hnest,
                    H1 into HnestC,
@@ -2196,7 +2191,7 @@ Module InterParse.
                            H5 into Hvs_fst,
                              vs0 into vs.
         rewrite map_to_list_insert_first_key by assumption.
-        simpl. (* rewrite filter_cons_True.
+        simpl. rewrite filter_cons_True.
         + f_equal. specialize (IHHsc vs eq_refl).
           fold (Vals (VALUE vs)). fold (ValList (DESC (<[k:=f]> ds)) (VALUE vs)).
           fold (Vals (VALUE vs)) in IHHsc. fold (ValList (DESC ds) (VALUE vs)) in IHHsc.
@@ -2207,8 +2202,6 @@ Module InterParse.
           destruct v; try trivial.
           destruct f; unfold field_val_type_match in Hty; assumption.
     Qed.
-                *)
-        Admitted.
 
     Lemma SC_Empty_Desc : forall d, ⟨ VALUE ∅ ∷ d ⟩ -> d = DESC ∅.
     Proof.
@@ -2226,17 +2219,15 @@ Module InterParse.
       induction vs as [| k v vs Hnone Hfst] using map_first_key_ind.
       - intros d Hsc. unfold ValList; simpl.
         apply SC_Empty_Desc in Hsc. subst. simpl.
-        rewrite merge_empty, map_to_list_empty.
+        rewrite map_to_list_empty, filter_nil.
         unfold list_to_value. done.
       - intros d Hsc.
         unfold ValList; simpl.
-        (*
         rewrite map_to_list_insert_first_key by assumption.
         rewrite filter_cons_True.
         + unfold list_to_value; simpl.
           assert (exists v', Vals (Init d) !! k = Some v') as Hdom. { admit. }
-          destruct Hdom as [v' Hdom]. rewrite Hdom.
-         *)
+          destruct Hdom as [v' Hdom]. 
     Abort.
 
     Lemma SC_filter_self : forall d v, ⟨ v ∷ d ⟩ -> ⟨ list_to_value d (ValList d v) ∷ d⟩.
@@ -2244,7 +2235,7 @@ Module InterParse.
       intros d v Hsc. apply SC_SCO in Hsc.
       induction Hsc as [| ? ? ? ? ? Hty Hnest HnestC Hds_no Hvs_no Hds_fst Hvs_fst].
       - unfold ValList; simpl.
-        rewrite merge_empty, map_to_list_empty.
+        rewrite map_to_list_empty, filter_nil.
         unfold list_to_value, foldl, Init.
         simpl. rewrite merge_empty.
         apply SC_Empty.
@@ -2272,36 +2263,23 @@ Module InterParse.
       intros v d Hsc. apply SC_SCO in Hsc.
       induction Hsc as [| ? ? ? ? ? Hty Hnest HnestC Hds_no Hvs_no Hds_fst Hvs_fst].
       - unfold ValList; simpl.
-        (*
         rewrite map_to_list_empty, filter_nil.
         unfold list_to_value, foldl, Init.
-        rewrite InitFold_eq.
-        rewrite map_fold_empty.
-        apply CompatRefl; apply SC_Empty.
+        (* rewrite InitFold_eq. *)
+        (* rewrite map_fold_empty. *)
+        (* apply CompatRefl; apply SC_Empty. *)
+        admit.
       - apply CompatibleEqual in IHHsc; last done.
         unfold ValList; simpl.
         rewrite map_to_list_insert_first_key by assumption.
         rewrite filter_cons_True. 
         + unfold list_to_value.
-          
-          apply CompatAdd.
+          admit.
         + unfold ValList_filter_p; simpl.
           rewrite lookup_insert_eq.
           destruct v; try trivial.
           unfold field_val_type_match in Hty.
           destruct f; contradiction.
-
-        apply CompatAdd with (k := k) (f1 := f) (f2 := f) (v'1 := v) (v'2 := v) in IHHsc; try done.
-        + autorewrite with desc_unfold in *; autorewrite with value_unfold in *.
-          simpl in IHHsc. admit.
-        + apply SC_SCO in Hsc. exact Hsc.
-        + inversion IHHsc; subst; first assumption.
-          destruct v1 as [vs1]; destruct v2 as [vs2].
-          destruct d1 as [ds1]; destruct d2 as [ds2].
-          autorewrite with value_unfold in *.
-          autorewrite with desc_unfold in *.
-          apply SC_insert_field with (k := k0) (f := f2) (v := v'2) in H4; try done.
-         *)
     Admitted.
 
     Definition ParseOk_Value_P (v : Value) :=
